Partially revert "Explicit namespaces for counter, lock and spawn."
In order to improve flexibility, I have reverted the changes in commit
5cabd278 to counter, lock and spawn because an explicit namespace may be in
the way of modularity, for example, if the interfaces of these libraries will
expose namespaces through view shifts in the future.

Exposure of namespaces in the case of par is very unlikely, so to that end,
par remains to use an explicit namespace.

heap_lang/lib/counter.v
@@ -5,8 +5,6 @@ From iris.proofmode Require Import invariants ghost_ownership coq_tactics.
 From iris.heap_lang Require Import proofmode notation.
 Import uPred.
 
-Definition counterN : namespace := nroot .@ "counter".
-
 Definition newcounter : val := λ: <>, ref #0.
 Definition inc : val :=
   rec: "inc" "l" :=
@@ -28,17 +26,19 @@ Local Notation iProp := (iPropG heap_lang Σ).
 Definition counter_inv (l : loc) (n : mnat) : iProp := (l ↦ #n)%I.
 
 Definition counter (l : loc) (n : nat) : iProp :=
-  (∃ γ, heap_ctx ∧ auth_ctx γ counterN (counter_inv l) ∧ auth_own γ (n:mnat))%I.
+  (∃ N γ, heapN ⊥ N ∧ heap_ctx ∧
+          auth_ctx γ N (counter_inv l) ∧ auth_own γ (n:mnat))%I.
 
 (** The main proofs. *)
 Global Instance counter_persistent l n : PersistentP (counter l n).
 Proof. apply _. Qed.
 
-Lemma newcounter_spec (R : iProp) Φ :
+Lemma newcounter_spec N (R : iProp) Φ :
+  heapN ⊥ N →
   heap_ctx ★ (∀ l, counter l 0 -★ Φ #l) ⊢ WP newcounter #() {{ Φ }}.
 Proof.
-  iIntros "[#Hh HΦ]". rewrite /newcounter. wp_seq. wp_alloc l as "Hl".
-  iPvs (auth_alloc (counter_inv l) counterN _ (O:mnat) with "[Hl]")
+  iIntros (?) "[#Hh HΦ]". rewrite /newcounter. wp_seq. wp_alloc l as "Hl".
+  iPvs (auth_alloc (counter_inv l) N _ (O:mnat) with "[Hl]")
     as (γ) "[#? Hγ]"; try by auto.
   iPvsIntro. iApply "HΦ". rewrite /counter; eauto 10.
 Qed.
@@ -47,13 +47,13 @@ Lemma inc_spec l j (Φ : val → iProp) :
   counter l j ★ (counter l (S j) -★ Φ #()) ⊢ WP inc #l {{ Φ }}.
 Proof.
   iIntros "[Hl HΦ]". iLöb as "IH". wp_rec.
-  iDestruct "Hl" as (γ) "(#Hh & #Hγ & Hγf)".
+  iDestruct "Hl" as (N γ) "(% & #? & #Hγ & Hγf)".
   wp_focus (! _)%E.
-  iApply (auth_fsa (counter_inv l) (wp_fsa _) _ counterN); auto with fsaV.
+  iApply (auth_fsa (counter_inv l) (wp_fsa _) _ N); auto with fsaV.
   iIntros "{$Hγ $Hγf}"; iIntros (j') "[% Hl] /="; rewrite {2}/counter_inv.
   wp_load; iPvsIntro; iExists j; iSplit; [done|iIntros "{$Hl} Hγf"].
   wp_let; wp_op. wp_focus (CAS _ _ _).
-  iApply (auth_fsa (counter_inv l) (wp_fsa _) _ counterN); auto with fsaV.
+  iApply (auth_fsa (counter_inv l) (wp_fsa _) _ N); auto with fsaV.
   iIntros "{$Hγ $Hγf}"; iIntros (j'') "[% Hl] /="; rewrite {2}/counter_inv.
   destruct (decide (j `max` j'' = j `max` j')) as [Hj|Hj].
   - wp_cas_suc; first (by do 3 f_equal); iPvsIntro.
@@ -62,7 +62,7 @@ Proof.
     rewrite {2}/counter_inv !mnat_op_max (Nat.max_l (S _)); last abstract lia.
     rewrite Nat2Z.inj_succ -Z.add_1_l.
     iIntros "{$Hl} Hγf". wp_if.
-    iPvsIntro; iApply "HΦ"; iExists γ; repeat iSplit; eauto.
+    iPvsIntro; iApply "HΦ"; iExists N, γ; repeat iSplit; eauto.
     iApply (auth_own_mono with "Hγf"). apply mnat_included. abstract lia.
   - wp_cas_fail; first (rewrite !mnat_op_max; by intros [= ?%Nat2Z.inj]).
     iPvsIntro. iExists j; iSplit; [done|iIntros "{$Hl} Hγf"].
@@ -73,9 +73,9 @@ Lemma read_spec l j (Φ : val → iProp) :
   counter l j ★ (∀ i, ■ (j ≤ i)%nat → counter l i -★ Φ #i)
   ⊢ WP read #l {{ Φ }}.
 Proof.
-  iIntros "[Hc HΦ]". iDestruct "Hc" as (γ) "(#Hh & #Hγ & Hγf)".
+  iIntros "[Hc HΦ]". iDestruct "Hc" as (N γ) "(% & #? & #Hγ & Hγf)".
   rewrite /read. wp_let.
-  iApply (auth_fsa (counter_inv l) (wp_fsa _) _ counterN); auto with fsaV.
+  iApply (auth_fsa (counter_inv l) (wp_fsa _) _ N); auto with fsaV.
   iIntros "{$Hγ $Hγf}"; iIntros (j') "[% Hl] /=".
   wp_load; iPvsIntro; iExists (j `max` j'); iSplit.
   { iPureIntro; apply mnat_local_update; abstract lia. }
